refactoring

src/SolinasReduction.v
@@ -89,18 +89,6 @@ Module solinas_reduction.
       Definition is_bounded_by bounds ls :=
         fold_andb_map' (fun r v'' => (fst r <=? v'') && (v'' <=? snd r)) bounds ls.
 
-      Definition mul_no_reduce base n (p q : list Z) :=
-        let p_a := Positional.to_associational weight n p in
-        let q_a := Positional.to_associational weight n q in
-        let pq_a := Saturated.Associational.sat_mul base p_a q_a in
-        let pq_rows := Saturated.Rows.from_associational weight (2*n) pq_a in
-        let pq := Saturated.Rows.flatten weight (2*n) pq_rows in
-        let bound := (0, 2^machine_wordsize - 1) in
-        if (is_bounded_by (repeat bound n) p && is_bounded_by (repeat bound n) q) then
-          fst pq
-        else
-          add_to_nth 0 (weight (2 * n) * snd pq) (fst pq).
-
       Definition sat_reduce base s c n (p : list (Z * Z)) :=
         let s' := fst (Saturated.Rows.adjust_s weight (S (S n)) s) in
         let lo_hi := Associational.split s' p in
@@ -118,32 +106,32 @@ Module solinas_reduction.
         fst r_flat.
 
       Definition reduce_full base s c n (p : list Z) :=
-        let r1 := reduce1 base s c (2*n) (S n) p in
         let bound := (0, 2^machine_wordsize - 1) in
-        let bounds := repeat bound n ++ [(0, up_bound-1)] in
-        if (is_bounded_by bounds r1) then
-          let r2 := reduce1 base s c (S n) (S n) r1 in
-          let r3 := reduce1 base s c (S n) (n) r2 in
-          r3
-        else r1.
-
-      (* Definition mulmod base s c n (p q : list Z) := *)
-      (*   let prod := mul_no_reduce base n p q in *)
-      (*   let red := reduce_full base s c n prod in *)
-      (*   red. *)
-
-      Definition mulmod base s c n (p q : list Z) :=
-        let p_a := Positional.to_associational weight n p in
-        let q_a := Positional.to_associational weight n q in
-        let pq_a := Saturated.Associational.sat_mul base p_a q_a in
-        let pq_rows := Saturated.Rows.from_associational weight (2*n) pq_a in
-        let pq := Saturated.Rows.flatten weight (2*n) pq_rows in
-        let bound := (0, 2^machine_wordsize - 1) in
-        if (is_bounded_by (repeat bound n) p && is_bounded_by (repeat bound n) q) then
-          let mul := fst pq in
-          reduce_full base s c n mul
+        if (is_bounded_by (repeat bound (2*n)) p) then
+          let r1 := reduce1 base s c (2*n) (S n) p in
+          if (is_bounded_by (repeat bound n ++ [(0, up_bound-1)]) r1) then
+            let r2 := reduce1 base s c (S n) (S n) r1 in
+            let r3 := reduce1 base s c (S n) (n) r2 in
+            r3
+          else r1
         else
-          repeat 0 n.
+          (* reduce down to n limbs *)
+          let p_a := Positional.to_associational weight n p in
+          let r_a := sat_reduce base s c n p_a in
+          let r_rows := Saturated.Rows.from_associational weight n r_a in
+          let r_flat := Saturated.Rows.flatten weight n r_rows in
+          add_to_nth 0 (weight (n) * snd r_flat) (fst r_flat).
+
+      Definition reduce1' base s c n m (p : list Z) :=
+        let p_a := Positional.to_associational weight n p in
+        let r_a := sat_reduce base s c n p_a in
+        let r_rows := Saturated.Rows.from_associational weight m r_a in
+        let r_flat := Saturated.Rows.flatten weight m r_rows in
+        let bound := (0, 2^machine_wordsize - 1) in
+        if (is_bounded_by (repeat bound n) p) then
+          fst r_flat
+        else
+          add_to_nth 0 (weight (m) * snd r_flat) (fst r_flat).
 
     End __.
 
@@ -155,11 +143,8 @@ Module solinas_reduction.
       Let n : nat := Z.to_nat (Qceiling (Z.log2_up s / machine_wordsize)).
       Let m : nat := 2 * n.
       Let w : nat -> Z := weight machine_wordsize 1.
+      Let up_bound := 2 ^ (machine_wordsize / 4).
       Let base : Z := 2 ^ machine_wordsize.
-
-      Let bound := Some r[0 ~> (2^machine_wordsize - 1)]%zrange.
-      Let boundsn : list (ZRange.type.option.interp base.type.Z)
-          := repeat bound (n).
 
       Import Stringification.C.Compilers.
       Import Stringification.C.Compilers.ToString.
@@ -183,6 +168,8 @@ Module solinas_reduction.
       Local Instance : split_mul_to_opt := split_mul_to_of_should_split_mul machine_wordsize possible_values.
       Local Instance : split_multiret_to_opt := split_multiret_to_of_should_split_multiret machine_wordsize possible_values.
 
+      Let bound := Some r[0 ~> (2^machine_wordsize - 1)]%zrange.
+      Let bound' := Some (repeat bound (n) ++ [Some r[0 ~> 1]%zrange]).
       Time Compute
            Show.show
            (Pipeline.BoundsPipelineToString
@@ -193,246 +180,52 @@ Module solinas_reduction.
               possible_values
               machine_wordsize
               ltac:(let n := (eval cbv in n) in
-                    let r := Reify (mulmod base s c n) in
+                    let r := Reify (reduce1' base s c (2*n) (S n)) in
                     exact r)
                      (fun _ _ => [])
-                     (Some (repeat bound n), (Some (repeat bound n), tt))
-                     (Some (repeat bound (n)))
-                     (None, (None, tt))
+                     (Some (repeat bound (2*n)), tt)
+                     (Some (repeat bound (S n)))
+                     (None, tt)
                      (None)
              : Pipeline.ErrorT _).
-
-    (*
-     = "Success (""/*
- * Input Bounds:
- *   arg1: [[0x0 ~> 0xffffffffffffffff], [0x0 ~> 0xffffffffffffffff], [0x0 ~> 0xffffffffffffffff], [0x0 ~> 0xffffffffffffffff]]
- *   arg2: [[0x0 ~> 0xffffffffffffffff], [0x0 ~> 0xffffffffffffffff], [0x0 ~> 0xffffffffffffffff], [0x0 ~> 0xffffffffffffffff]]
- * Output Bounds:
- *   out1: [[0x0 ~> 0xffffffffffffffff], [0x0 ~> 0xffffffffffffffff], [0x0 ~> 0xffffffffffffffff], [0x0 ~> 0xffffffffffffffff]]
- */
-static void mul(uint64_t out1[4], const uint64_t arg1[4], const uint64_t arg2[4]) {
-  uint64_t x1;
-  uint64_t x2;
-  uint64_t x3;
-  uint64_t x4;
-  uint64_t x5;
-  uint64_t x6;
-  uint64_t x7;
-  uint64_t x8;
-  uint64_t x9;
-  uint64_t x10;
-  uint64_t x11;
-  uint64_t x12;
-  uint64_t x13;
-  uint64_t x14;
-  uint64_t x15;
-  uint64_t x16;
-  uint64_t x17;
-  uint64_t x18;
-  uint64_t x19;
-  uint64_t x20;
-  uint64_t x21;
-  uint64_t x22;
-  uint64_t x23;
-  uint64_t x24;
-  uint64_t x25;
-  uint64_t x26;
-  uint64_t x27;
-  uint64_t x28;
-  uint64_t x29;
-  uint64_t x30;
-  uint64_t x31;
-  uint64_t x32;
-  uint64_t x33;
-  fiatuint1 x34;
-  uint64_t x35;
-  fiatuint1 x36;
-  uint64_t x37;
-  uint64_t x38;
-  fiatuint1 x39;
-  uint64_t x40;
-  fiatuint1 x41;
-  uint64_t x42;
-  fiatuint1 x43;
-  uint64_t x44;
-  uint64_t x45;
-  fiatuint1 x46;
-  uint64_t x47;
-  fiatuint1 x48;
-  uint64_t x49;
-  fiatuint1 x50;
-  uint64_t x51;
-  fiatuint1 x52;
-  uint64_t x53;
-  fiatuint1 x54;
-  uint64_t x55;
-  uint64_t x56;
-  fiatuint1 x57;
-  uint64_t x58;
-  fiatuint1 x59;
-  uint64_t x60;
-  fiatuint1 x61;
-  uint64_t x62;
-  fiatuint1 x63;
-  uint64_t x64;
-  fiatuint1 x65;
-  uint64_t x66;
-  fiatuint1 x67;
-  uint64_t x68;
-  fiatuint1 x69;
-  uint64_t x70;
-  fiatuint1 x71;
-  uint64_t x72;
-  fiatuint1 x73;
-  uint64_t x74;
-  fiatuint1 x75;
-  uint64_t x76;
-  fiatuint1 x77;
-  uint64_t x78;
-  fiatuint1 x79;
-  uint64_t x80;
-  fiatuint1 x81;
-  uint64_t x82;
-  fiatuint1 x83;
-  uint64_t x84;
-  fiatuint1 x85;
-  uint64_t x86;
-  fiatuint1 x87;
-  uint64_t x88;
-  fiatuint1 x89;
-  uint64_t x90;
-  fiatuint1 x91;
-  uint64_t x92;
-  fiatuint1 x93;
-  uint64_t x94;
-  fiatuint1 x95;
-  uint64_t x96;
-  uint64_t x97;
-  uint64_t x98;
-  uint64_t x99;
-  uint64_t x100;
-  uint64_t x101;
-  uint64_t x102;
-  fiatuint1 x103;
-  uint64_t x104;
-  fiatuint1 x105;
-  uint64_t x106;
-  uint64_t x107;
-  uint64_t x108;
-  fiatuint1 x109;
-  uint64_t x110;
-  uint64_t x111;
-  uint64_t x112;
-  uint64_t x113;
-  fiatuint1 x114;
-  uint64_t x115;
-  fiatuint1 x116;
-  uint64_t x117;
-  fiatuint1 x118;
-  uint64_t x119;
-  fiatuint1 x120;
-  uint64_t x121;
-  uint64_t x122;
-  uint64_t x123;
-  uint64_t x124;
-  fiatuint1 x125;
-  uint64_t x126;
-  fiatuint1 x127;
-  uint64_t x128;
-  fiatuint1 x129;
-  uint64_t x130;
-  fiatuint1 x131;
-  uint64_t x132;
-  uint64_t x133;
-  uint64_t x134;
-  fiatuint1 x135;
-  uint64_t x136;
-  fiatuint1 x137;
-  uint64_t x138;
-  fiatuint1 x139;
-  uint64_t x140;
-  fiatuint1 x141;
-  fiatmulx_u64(&x1, &x2, (arg1[3]), (arg2[3]));
-  fiatmulx_u64(&x3, &x4, (arg1[3]), (arg2[2]));
-  fiatmulx_u64(&x5, &x6, (arg1[3]), (arg2[1]));
-  fiatmulx_u64(&x7, &x8, (arg1[3]), (arg2[0]));
-  fiatmulx_u64(&x9, &x10, (arg1[2]), (arg2[3]));
-  fiatmulx_u64(&x11, &x12, (arg1[2]), (arg2[2]));
-  fiatmulx_u64(&x13, &x14, (arg1[2]), (arg2[1]));
-  fiatmulx_u64(&x15, &x16, (arg1[2]), (arg2[0]));
-  fiatmulx_u64(&x17, &x18, (arg1[1]), (arg2[3]));
-  fiatmulx_u64(&x19, &x20, (arg1[1]), (arg2[2]));
-  fiatmulx_u64(&x21, &x22, (arg1[1]), (arg2[1]));
-  fiatmulx_u64(&x23, &x24, (arg1[1]), (arg2[0]));
-  fiatmulx_u64(&x25, &x26, (arg1[0]), (arg2[3]));
-  fiatmulx_u64(&x27, &x28, (arg1[0]), (arg2[2]));
-  fiatmulx_u64(&x29, &x30, (arg1[0]), (arg2[1]));
-  fiatmulx_u64(&x31, &x32, (arg1[0]), (arg2[0]));
-  fiataddcarryx_u64(&x33, &x34, 0x0, x28, x7);
-  fiataddcarryx_u64(&x35, &x36, x34, x26, x5);
-  x37 = (x36 + x18);
-  fiataddcarryx_u64(&x38, &x39, 0x0, x33, x13);
-  fiataddcarryx_u64(&x40, &x41, x39, x35, x8);
-  fiataddcarryx_u64(&x42, &x43, x41, x37, 0x0);
-  x44 = (x43 + x10);
-  fiataddcarryx_u64(&x45, &x46, 0x0, x30, x15);
-  fiataddcarryx_u64(&x47, &x48, x46, x38, x16);
-  fiataddcarryx_u64(&x49, &x50, x48, x40, x11);
-  fiataddcarryx_u64(&x51, &x52, x50, x42, x3);
-  fiataddcarryx_u64(&x53, &x54, x52, x44, 0x0);
-  x55 = (x54 + x2);
-  fiataddcarryx_u64(&x56, &x57, 0x0, x45, x21);
-  fiataddcarryx_u64(&x58, &x59, x57, x47, x19);
-  fiataddcarryx_u64(&x60, &x61, x59, x49, x14);
-  fiataddcarryx_u64(&x62, &x63, x61, x51, x6);
-  fiataddcarryx_u64(&x64, &x65, x63, x53, 0x0);
-  fiataddcarryx_u64(&x66, &x67, x65, x55, 0x0);
-  fiataddcarryx_u64(&x68, &x69, 0x0, x32, x23);
-  fiataddcarryx_u64(&x70, &x71, x69, x56, x24);
-  fiataddcarryx_u64(&x72, &x73, x71, x58, x22);
-  fiataddcarryx_u64(&x74, &x75, x73, x60, x17);
-  fiataddcarryx_u64(&x76, &x77, x75, x62, x9);
-  fiataddcarryx_u64(&x78, &x79, x77, x64, x1);
-  fiataddcarryx_u64(&x80, &x81, x79, x66, 0x0);
-  fiataddcarryx_u64(&x82, &x83, 0x0, x68, x29);
-  fiataddcarryx_u64(&x84, &x85, x83, x70, x27);
-  fiataddcarryx_u64(&x86, &x87, x85, x72, x25);
-  fiataddcarryx_u64(&x88, &x89, x87, x74, x20);
-  fiataddcarryx_u64(&x90, &x91, x89, x76, x12);
-  fiataddcarryx_u64(&x92, &x93, x91, x78, x4);
-  fiataddcarryx_u64(&x94, &x95, x93, x80, 0x0);
-  fiatmulx_u64(&x96, &x97, UINT8_C(0x26), x92);
-  fiatmulx_u64(&x98, &x99, UINT8_C(0x26), x90);
-  fiatmulx_u64(&x100, &x101, UINT8_C(0x26), x88);
-  fiataddcarryx_u64(&x102, &x103, 0x0, x82, x98);
-  fiataddcarryx_u64(&x104, &x105, x103, x84, x96);
-  fiatmulx_u64(&x106, &x107, UINT8_C(0x26), x94);
-  fiataddcarryx_u64(&x108, &x109, x105, x86, x106);
-  fiatmulx_u64(&x110, &x111, UINT8_C(0x26), x94);
-  x112 = (x109 + x111);
-  fiataddcarryx_u64(&x113, &x114, 0x0, x31, x100);
-  fiataddcarryx_u64(&x115, &x116, x114, x102, x101);
-  fiataddcarryx_u64(&x117, &x118, x116, x104, x99);
-  fiataddcarryx_u64(&x119, &x120, x118, x108, x97);
-  x121 = (x120 + x112);
-  fiatmulx_u64(&x122, &x123, UINT8_C(0x26), x121);
-  fiataddcarryx_u64(&x124, &x125, 0x0, x113, x122);
-  fiataddcarryx_u64(&x126, &x127, x125, x115, 0x0);
-  fiataddcarryx_u64(&x128, &x129, x127, x117, 0x0);
-  fiataddcarryx_u64(&x130, &x131, x129, x119, 0x0);
-  fiatmulx_u64(&x132, &x133, UINT8_C(0x26), x131);
-  fiataddcarryx_u64(&x134, &x135, 0x0, x124, x132);
-  fiataddcarryx_u64(&x136, &x137, x135, x126, 0x0);
-  fiataddcarryx_u64(&x138, &x139, x137, x128, 0x0);
-  fiataddcarryx_u64(&x140, &x141, x139, x130, 0x0);
-  out1[0] = x134;
-  out1[1] = x136;
-  out1[2] = x138;
-  out1[3] = x140;
-}"", {| bitwidths_used := [uint1, uint64] ; addcarryx_lg_splits := [64] ; mulx_lg_splits := [64] ; cmovznz_bitwidths := [] ; value_barrier_bitwidths := [] ; typedefs_used := [] |})"
-     : string
-Finished transaction in 7.129 secs (6.859u,0.198s) (successful)
-     *)
+      Time Compute
+           Show.show
+           (Pipeline.BoundsPipelineToString
+              "fiat" "mul"
+              false
+              false
+              None
+              possible_values
+              machine_wordsize
+              ltac:(let n := (eval cbv in n) in
+                    let r := Reify (reduce_full base s c n) in
+                    exact r)
+                     (fun _ _ => [])
+                     (Some (repeat bound (2*n)), tt)
+                     (Some (repeat bound (n)))
+                     (None, tt)
+                     (None)
+             : Pipeline.ErrorT _).
+(* first reduction unnecessarily scales one of the limbs twice
+  fiatmulx_u64(&x1, &x2, UINT8_C(0x26), (arg1[6]));
+  fiatmulx_u64(&x3, &x4, UINT8_C(0x26), (arg1[5]));
+  fiatmulx_u64(&x5, &x6, UINT8_C(0x26), (arg1[4]));
+  x7 = (arg1[3]);
+  x8 = (arg1[2]);
+  x9 = (arg1[1]);
+  x10 = (arg1[0]);
+  fiataddcarryx_u64(&x11, &x12, 0x0, x9, x3);
+  fiataddcarryx_u64(&x13, &x14, x12, x8, x1);
+  fiatmulx_u64(&x15, &x16, UINT8_C(0x26), (arg1[7]));
+  fiataddcarryx_u64(&x17, &x18, x14, x7, x15);
+  fiatmulx_u64(&x19, &x20, UINT8_C(0x26), (arg1[7]));
+  x21 = (x18 + x20);
+  fiataddcarryx_u64(&x22, &x23, 0x0, x10, x5);
+  fiataddcarryx_u64(&x24, &x25, x23, x11, x6);
+  fiataddcarryx_u64(&x26, &x27, x25, x13, x4);
+  fiataddcarryx_u64(&x28, &x29, x27, x17, x2);
+  x30 = (x29 + x21);
+       *)
 
     End __.
 
@@ -446,12 +239,12 @@ Finished transaction in 7.129 secs (6.859u,0.198s) (successful)
             {wprops : @weight_properties weight}.
 
     Ltac weight_comp :=
-      unfold weight, uweight, ModOps.weight;
-      rewrite !Z.div_1_r;
-      rewrite !Z.opp_involutive;
-      try rewrite Nat2Z.inj_succ;
-      try rewrite OrdersEx.Z_as_OT.mul_succ_r;
-      try rewrite OrdersEx.Z_as_OT.pow_add_r;
+      unfold weight, uweight, ModOps.weight, machine_wordsize;
+      try rewrite !Z.div_1_r;
+      try rewrite !Z.opp_involutive;
+      try rewrite !Nat2Z.inj_succ;
+      try rewrite !OrdersEx.Z_as_OT.mul_succ_r;
+      try rewrite !OrdersEx.Z_as_OT.pow_add_r;
       autorewrite with zsimplify_const;
       ring_simplify.
 
@@ -463,6 +256,9 @@ Finished transaction in 7.129 secs (6.859u,0.198s) (successful)
         | _ => apply OrdersEx.Z_as_OT.mul_pos_pos
         | _ => apply OrdersEx.Z_as_OT.div_pos
         | _ => apply OrdersEx.Z_as_OT.div_lt_upper_bound
+        | _ => apply Z.mod_small
+        | |- _ - ?x < _ - ?x => rewrite <-OrdersEx.Z_as_OT.sub_lt_mono_r
+        | |- _ - ?x <= _ - ?x => rewrite <-OrdersEx.Z_as_OT.sub_le_mono_r
         | |- _ mod (?x * ?y) < (?y * ?x) => rewrite Z.mul_comm with (n:=x)
         | _ => apply OrdersEx.Z_as_OT.mod_pos_bound
 
@@ -475,6 +271,10 @@ Finished transaction in 7.129 secs (6.859u,0.198s) (successful)
         | _ => lia
         end.
 
+    Ltac le_lt :=
+      (rewrite Le.Z.le_sub_1_iff || rewrite <-Le.Z.le_sub_1_iff).
+
+    Hint Rewrite eval_cons using auto : push_eval.
     Hint Rewrite Associational.eval_sat_mul using lia : push_eval.
     Hint Rewrite Associational.eval_sat_mul_const using lia : push_eval.
     Hint Rewrite eval_split using auto : push_eval.
@@ -482,27 +282,52 @@ Finished transaction in 7.129 secs (6.859u,0.198s) (successful)
     Hint Rewrite Rows.flatten_mod using (eauto using Rows.length_from_associational) : push_eval.
     Hint Rewrite Rows.flatten_correct using (eauto using Rows.length_from_associational) : push_eval.
     Hint Rewrite eval_add_to_nth using auto : push_eval.
-    Hint Rewrite (@fst_pair) : push_eval.
-    Hint Rewrite (@snd_pair) : push_eval.
 
+    Hint Rewrite cons_length : push_length.
     Hint Rewrite app_length : push_length.
     Hint Rewrite (@ListUtil.length_snoc) : push_length.
     Hint Rewrite (@nil_length0) : push_length.
     Hint Rewrite seq_length : push_length.
     Hint Rewrite map_length : push_length.
     Hint Rewrite firstn_length : push_length.
+    Hint Rewrite @skipn_length : push_length.
     Hint Rewrite Rows.length_flatten using (eauto using Rows.length_from_associational) : push_length.
     Hint Rewrite length_partition : push_length.
+    Hint Rewrite length_add_to_nth : push_length.
 
     Hint Rewrite map_app : push_misc.
     Hint Rewrite (@combine_app_samelength) using (autorewrite with push_length; lia) : push_misc.
+    Hint Rewrite @combine_nil_r : push_misc.
     Hint Rewrite fold_right_app : push_misc.
     Hint Rewrite (@firstn_map) : push_misc.
     Hint Rewrite firstn_seq : push_misc.
+    Hint Rewrite seq_add : push_misc.
     Hint Rewrite map_map : push_misc.
     Hint Rewrite <-seq_shift : push_misc.
+    Hint Rewrite in_map_iff : push_misc.
+    Hint Rewrite firstn_app : push_misc.
+    Hint Rewrite @skipn_app : push_misc.
+    Hint Rewrite @skipn_0 : push_misc.
+    Hint Rewrite (@fst_pair) : push_misc.
+    Hint Rewrite (@snd_pair) : push_misc.
+    Hint Rewrite Nat.sub_diag : push_misc.
+    Hint Rewrite app_nil_r : push_misc.
+    Hint Rewrite app_nil_l : push_misc.
 
-    Ltac push := autorewrite with push_eval push_length push_misc.
+    Hint Resolve in_or_app : core.
+    Hint Resolve in_eq : core.
+    Hint Resolve in_cons : core.
+
+    Ltac push :=
+      autorewrite with push_eval push_length push_misc zsimplify_const;
+      auto.
+
+    Lemma seq_double : forall n,
+        seq 0 (2 * n) = seq 0 n ++ seq n n.
+    Proof.
+      intros n; replace (2*n)%nat with (n+n)%nat; push; lia.
+    Qed.
+    Hint Rewrite seq_double : push_misc.
 
     Section canon.
 
@@ -538,7 +363,7 @@ Finished transaction in 7.129 secs (6.859u,0.198s) (successful)
                      destruct H as [ Hlen Hpart ]
                  | H1 : In _ ?p, H2 : ?p = _ |- _ =>
                      rewrite H2 in H1;
-                     rewrite in_map_iff in H1
+                     autorewrite with push_misc in H1
                  | H : context[exists _, _] |- _ => destruct H
                  | H : _ = ?x |- 0 <= ?x => rewrite <-H
                  | H : _ = ?x |- ?x < _ => rewrite <-H
@@ -578,7 +403,12 @@ Finished transaction in 7.129 secs (6.859u,0.198s) (successful)
       Proof.
         intros.
         rewrite canonical_iff in *.
-        intuition; apply H1; simpl; eauto.
+        intuition;
+          repeat multimatch goal with
+                 | H : context[_ <= _ < _] |- _ => apply H
+                 | _ => cbn
+                 | _ => auto
+                 end.
       Qed.
 
       Lemma canonical_app_l n n1 n2 l l1 l2 :
@@ -590,9 +420,13 @@ Finished transaction in 7.129 secs (6.859u,0.198s) (successful)
         canonical_repr n1 l1.
       Proof.
         intros.
-        intuition;
-          rewrite canonical_iff in *;
-          intuition; apply H5; rewrite H3; apply in_or_app; eauto.
+        rewrite canonical_iff in *; intuition;
+          repeat multimatch goal with
+                 | H : context[_ <= _ < _] |- _ => apply H
+                 | H : ?x = _ ++ _ |- In _ ?x => rewrite H
+                 | _ => cbn
+                 | _ => auto
+                 end.
       Qed.
 
       Lemma canonical_app_r n n1 n2 l l1 l2 :
@@ -604,15 +438,20 @@ Finished transaction in 7.129 secs (6.859u,0.198s) (successful)
         canonical_repr n2 l2.
       Proof.
         intros.
-        intuition;
-          rewrite canonical_iff in *;
-          intuition; apply H5; rewrite H3; apply in_or_app; eauto.
+        rewrite canonical_iff in *; intuition;
+          repeat multimatch goal with
+                 | H : context[_ <= _ < _] |- _ => apply H
+                 | H : ?x = _ ++ _ |- In _ ?x => rewrite H
+                 | _ => cbn
+                 | _ => auto
+                 end.
       Qed.
 
       Lemma fold_right_add : forall l x,
           fold_right Z.add x l = x + fold_right Z.add 0 l.
       Proof.
-        induction l; intros; cbn; try rewrite IHl; lia.
+        intros l x.
+        induction l as [ | l' IHl ]; cbn; try rewrite IHl; lia.
       Qed.
 
       Definition eval_weight_P p :=
@@ -625,44 +464,42 @@ Finished transaction in 7.129 secs (6.859u,0.198s) (successful)
       Proof.
         apply (ListAux.list_length_induction Z).
         unfold eval_weight_P.
-        intros.
+        intros l1 H n.
         pose proof (@break_list_last Z l1).
+                cbv [eval_weight_P eval Associational.eval to_associational] in *.
         intuition;
-          repeat match goal with
+          repeat multimatch goal with
                  | H : context[exists _, _] |- _ => destruct H
-                 | _ => rewrite eval_nil
+                 | _ => autorewrite with push_eval push_misc
                  | _ => progress subst
                  | _ => lia || auto
                  end.
-        cbv [eval_weight_P eval Associational.eval to_associational] in *.
+
         destruct (n <=? length x)%nat eqn:E.
         rewrite Nat.leb_le in E.
         rewrite combine_truncate_r.
         rewrite combine_truncate_r with (xs:=map weight (seq 0 (n))).
-        autorewrite with push_length.
+        push.
         apply H.
-        autorewrite with push_length.
+        push.
         rewrite Nat.min_l; lia.
 
         rewrite Nat.leb_gt in E.
         rewrite combine_truncate_l.
         rewrite combine_truncate_l with (xs:=map weight (seq 0 n)).
         autorewrite with push_length push_misc.
-        rewrite Nat.min_l.
+        rewrite Nat.min_l; [|lia].
         rewrite seq_snoc.
         autorewrite with push_misc.
         cbn.
-
         rewrite fold_right_add.
         rewrite fold_right_add with (x:=weight (Datatypes.length x) * x0 + 0).
         rewrite H.
         ring_simplify.
         unfold weight, machine_wordsize.
-        rewrite uweight_S.
-        cbn; break_match; try lia.
-        lia.
-        autorewrite with push_length; lia.
-        lia.
+        rewrite uweight_S; [|lia].
+        cbn; break_match; lia.
+        push.
       Qed.
 
       Lemma eval_weight_S p n:
@@ -673,64 +510,40 @@ Finished transaction in 7.129 secs (6.859u,0.198s) (successful)
         unfold eval_weight_P in *.
         auto.
       Qed.
+      Hint Rewrite eval_weight_S : push_eval.
 
       Lemma canonical_eval_bounded n : forall (p : list Z),
           canonical_repr n p ->
           eval weight n p < weight n.
       Proof.
-        intros.
-        pose proof (canonical_bounded _ _ H).
-        assert (Hcanon: canonical_repr n p) by assumption.
-        unfold canonical_repr in H; intuition.
+        intros p.
         generalize dependent n.
-        induction p; intros.
-        { simpl in H1; subst.
-          vm_compute.
-          eauto. }
-        { simpl in H1; subst.
-          rewrite eval_cons.
-          autorewrite with zsimplify_const.
-          rewrite eval_weight_S.
-          assert (a + eval weight (Datatypes.length p) p * weight 1 < 2^machine_wordsize + eval weight (Datatypes.length p) p * weight 1).
-          rewrite <-OrdersEx.Z_as_OT.add_lt_mono_r.
-          apply H0.
-          simpl.
-          left.
-          reflexivity.
-          rewrite <-Le.Z.le_sub_1_iff.
-          rewrite <-Le.Z.le_sub_1_iff in H.
-          etransitivity.
-          apply H.
-          assert (2 ^ machine_wordsize + eval weight (Datatypes.length p) p * weight 1 <= 2 ^ machine_wordsize + (weight (Datatypes.length p) - 1) * weight 1).
-          rewrite <-OrdersEx.Z_as_OT.add_le_mono_l.
-          rewrite <-OrdersEx.Z_as_OT.mul_le_mono_pos_r.
-          rewrite Le.Z.le_sub_1_iff.
-          apply IHp.
-          intros.
-          apply H0.
-          simpl.
-          eauto.
-          eapply canonical_cons; eauto.
-          reflexivity.
-          apply canonical_cons in Hcanon.
-          unfold canonical_repr in Hcanon.
-        intuition.
-        apply wprops.
-        rewrite OrdersEx.Z_as_OT.sub_le_mono_r with (p:=1) in H1.
+        induction p; intros; destruct n;
+          repeat multimatch goal with
+                 | H : canonical_repr _ (_ :: _) |- _ =>
+                     let H' := fresh "H" in
+                     assert (H' := H);
+                     pose proof (canonical_bounded _ _ H');
+                     unfold canonical_repr in H';
+                     apply canonical_cons in H
+                 | H : context[length _] |- _ => autorewrite with push_length in H; rewrite <-H
+                 | _ => push
+                 | _ => intuition
+                 | _ => ring_simplify
+                 | _ => auto || lia
+                 end.
+        cbn; lia.
+        le_lt.
         etransitivity.
-        apply H1.
-        weight_comp.
-        rewrite <-OrdersEx.Z_as_OT.sub_le_mono_r.
-        rewrite Nat2Z.inj_succ.
-        rewrite OrdersEx.Z_as_OT.mul_succ_r.
-        rewrite OrdersEx.Z_as_OT.pow_add_r.
+        solve_ineq.
+        le_lt.
+        apply H1; auto.
+        rewrite <-OrdersEx.Z_as_OT.mul_le_mono_pos_r; auto.
+        le_lt; auto.
         ring_simplify.
-        reflexivity.
-        lia.
-        lia.
-        lia.
-        lia.
-        lia. }
+        solve_ineq.
+        rewrite H2.
+        weight_comp; lia.
       Qed.
 
       Definition dual_map {A B : Type} (f : A -> B -> bool) (l1 : list A) (l2 : list B) :=
@@ -825,19 +638,14 @@ Finished transaction in 7.129 secs (6.859u,0.198s) (successful)
                  | _ => progress cbn || intuition
                  | _ => lia || auto || reflexivity || discriminate
                  end.
-        rewrite <-Le.Z.le_sub_1_iff.
+        le_lt.
         etransitivity.
         solve_ineq.
         break_match; eauto.
-        apply OrdersEx.Z_as_OT.mul_le_mono_nonneg_r.
-        lia.
-        rewrite Le.Z.le_sub_1_iff.
+        apply OrdersEx.Z_as_OT.mul_le_mono_nonneg_r; try lia.
+        le_lt.
         apply IHp; auto.
-        weight_comp.
-        unfold machine_wordsize.
-        lia.
-        lia.
-        lia.
+        weight_comp; unfold machine_wordsize; lia.
       Qed.
 
     End canon.
@@ -950,6 +758,7 @@ Finished transaction in 7.129 secs (6.859u,0.198s) (successful)
       intros; cbv [sat_reduce] in *; cbv [s' lo_hi coef].
       autorewrite with push_eval; lia.
     Qed.
+    Hint Rewrite value_sat_reduce : push_eval.
 
     Lemma adjust_s_invariant fuel s (s_nz:s<>0) :
       fst (Saturated.Rows.adjust_s weight fuel s) mod s = 0
@@ -1025,12 +834,6 @@ Finished transaction in 7.129 secs (6.859u,0.198s) (successful)
       let r_flat := Saturated.Rows.flatten weight m r_rows in
       fst r_flat.
 
-    Definition reduce base s c n (p : list Z) :=
-      let r1 := reduce1 base s c (2*n) (S n) p in
-      let r2 := reduce1 base s c (S n) (S n) (r1) in
-      let r3 := reduce1 base s c (S n) (n) (r2) in
-      r3.
-
     Definition reduce_full base s c n (p : list Z) :=
       let r1 := reduce1 base s c (2*n) (S n) p in
       let bound := (0, 2^machine_wordsize - 1) in
@@ -1056,35 +859,27 @@ Finished transaction in 7.129 secs (6.859u,0.198s) (successful)
     Proof.
       intros.
       generalize dependent l2.
-      induction l1; intros.
-      { reflexivity. }
-      { simpl.
-        destruct l2 eqn:E.
-        simpl in H0.
-        discriminate.
-        match goal with
-        | [ |- context[ ?x :: ?y ] ] => replace (x :: y) with ([x] ++ y) by eauto
-        end.
-        rewrite split_app.
-        rewrite IHl1.
-        cbn [fst snd].
-        simpl.
-        assert (In a (a :: l1)) by apply in_eq.
-        apply H in H1.
-        assert (a mod w = a).
-        { apply Z.mod_small.
-          lia. }
-        rewrite H2.
-        destruct (a =? 0) eqn:E1.
-        rewrite Z.eqb_eq in E1.
-        lia.
-        reflexivity.
-        intros.
-        apply H.
-        apply in_cons.
-        assumption.
-        simpl in H0.
-        lia. }
+      induction l1; intros; destruct l2;
+        repeat multimatch goal with
+               | _ => push
+               | _ => cbn
+               | _ => auto
+               end.
+
+      match goal with
+      | [ |- context[ ?x :: ?y ] ] => replace (x :: y) with ([x] ++ y) by eauto
+      end.
+      rewrite split_app.
+      pose proof (H a ltac:(auto)).
+      rewrite IHl1.
+      cbn.
+      replace (a mod w) with a.
+      destruct (a =? 0) eqn:E.
+      lia.
+      reflexivity.
+      rewrite Z.mod_small; lia.
+      auto.
+      auto.
     Qed.
 
     Lemma split_gt w l1 l2:
@@ -1159,6 +954,17 @@ Finished transaction in 7.129 secs (6.859u,0.198s) (successful)
       lia.
     Qed.
 
+    Lemma weight_mono_le x1 x2 :
+      (x1 <= x2)%nat ->
+      weight x1 <= weight x2.
+    Proof.
+      intros H.
+      apply le_lt_or_eq in H.
+      intuition.
+      pose proof (weight_mono x1 x2 ltac:(auto)); lia.
+      subst; lia.
+    Qed.
+
     Context (base : Z)
             (s : Z)
             (c : list (Z * Z))
@@ -1172,210 +978,296 @@ Finished transaction in 7.129 secs (6.859u,0.198s) (successful)
             (solinas_property : Rows.adjust_s weight (S (S n)) s = (weight n, true))
             (coef_small : weight n / s * Associational.eval c < up_bound).
 
-    Theorem eval_mul_no_reduce : forall p q,
-        Positional.eval weight (2 * n) (mul_no_reduce base n p q) =
-          Positional.eval weight n p * Positional.eval weight n q.
-    Proof using base_nz n_gt_1 wprops.
-      intros.
-      cbv [mul_no_reduce].
-      break_match.
-      (* properly bounded *)
-      autorewrite with push_eval.
-      apply Z.mod_small.
-      repeat match goal with
-             | H : context[_ && _] |- _ => rewrite andb_true_iff in Heqb
-             | H : is_bounded_by _ _ = true |- _ => apply eval_is_bounded_by in H
-             | _ => progress intuition
-             | _ => solve_ineq
-             end.
-      rewrite <-Le.Z.le_sub_1_iff.
-      etransitivity.
-      apply OrdersEx.Z_as_OT.mul_le_mono_nonneg; eauto; rewrite Le.Z.le_sub_1_iff; eauto.
-      rewrite Le.Z.le_sub_1_iff.
-      replace (weight (2 * n)) with (weight n * weight n).
-      solve_ineq.
-      weight_comp.
-      rewrite <-OrdersEx.Z_as_OT.pow_mul_r.
-      f_equal.
-      lia.
-      lia.
-      lia.
+    Section mul_no_reduce.
 
-      (* not bounded *)
-      push.
-      ring_simplify.
-      rewrite <-Z_div_mod_eq.
-      auto.
-      rewrite Z.gt_lt_iff.
-      auto.
-      push.
-      lia.
-      push.
-      lia.
-    Qed.
-
-    Lemma split_p : forall p lo hi,
-        p = lo ++ [hi] ->
-        canonical_repr (S n) p ->
-        (split (weight n) [(weight n, hi)] = ([], [(1, hi)])) /\
-          (split (weight n) (combine (map weight (seq 0 n)) lo) =
-             ((combine (map weight (seq 0 n)) lo), [])).
-    Proof.
-      intros.
-      intuition.
-      { intros.
-        unfold split.
-        simpl.
-        assert (weight n mod weight n = 0) by (apply Z_mod_same_full).
-        rewrite H1.
-        simpl.
-        assert (weight n / weight n = 1) by
-          auto using Z_div_same, Z.lt_gt, weight_positive.
-        rewrite H2.
-        reflexivity. }
-      { apply split_lt.
+      Theorem eval_mul_no_reduce : forall p q,
+          Positional.eval weight (2 * n) (mul_no_reduce base n p q) =
+            Positional.eval weight n p * Positional.eval weight n q.
+      Proof using base_nz n_gt_1 wprops.
         intros.
-        rewrite in_map_iff in H1.
-        destruct H1.
-        intuition.
-        rewrite <-H2.
-        auto.
-        rewrite <-H2.
-        rewrite in_seq in H3.
-        intuition.
-        simpl in H4.
-        apply weight_mono.
-        lia.
-        rewrite map_length.
-        rewrite seq_length.
-        solve_length p. }
-    Qed.
-
-    Lemma reduce_in_range : forall m x,
-        x < weight 1 - weight 0 ->
-        x + weight m < weight (S m).
-    Proof.
-      intros.
-      rewrite OrdersEx.Z_as_DT.lt_add_lt_sub_r.
-      induction m.
-      auto.
-      etransitivity.
-      apply IHm.
-      unfold weight.
-      rewrite uweight_S.
-      rewrite uweight_S.
-      rewrite <-uweight_S at 1.
-      rewrite <-OrdersEx.Z_as_OT.mul_sub_distr_l.
-      rewrite Z.mul_comm.
-      rewrite <-OrdersEx.Z_as_OT.lt_mul_diag_r.
-      simpl; lia.
-      rewrite OrdersEx.Z_as_OT.lt_0_sub.
-      fold weight.
-      apply weight_mono'.
-      lia.
-      lia.
-      lia.
-    Qed.
-
-    Lemma map_weight_seq : forall m p,
-        map weight (seq 0 p) = map (fun t => t / (weight m)) (map weight (seq m p)).
-    Proof.
-      induction m; intros.
-      { generalize dependent (map weight (seq 0 p)).
-        intros.
-        erewrite map_ext.
-        symmetry.
-        eapply map_id.
-        intros.
-        rewrite weight_0.
-        rewrite Z.div_1_r.
-        lia.
-        auto. }
-      { rewrite IHm.
-        rewrite <-map_S_seq.
-        rewrite !map_map.
-        apply map_ext_Forall.
-        rewrite Forall_forall.
-        intros.
-        rewrite in_seq in H.
+        cbv [mul_no_reduce].
+        break_match.
+        (* properly bounded *)
+        push.
+        apply Z.mod_small.
+        repeat match goal with
+               | H : context[_ && _] |- _ => rewrite andb_true_iff in Heqb
+               | H : is_bounded_by _ _ = true |- _ => apply eval_is_bounded_by in H
+               | _ => progress intuition
+               | _ => solve_ineq
+               end.
+        le_lt.
+        etransitivity.
+        apply OrdersEx.Z_as_OT.mul_le_mono_nonneg; eauto; rewrite Le.Z.le_sub_1_iff; eauto.
+        le_lt.
+        replace (weight (2 * n)) with (weight n * weight n).
+        solve_ineq.
         weight_comp.
-        rewrite <-OrdersEx.Z_as_OT.pow_add_r.
-        rewrite <- !OrdersEx.Z_as_OT.pow_sub_r.
+        rewrite <-OrdersEx.Z_as_OT.pow_mul_r.
         f_equal.
         lia.
         lia.
         lia.
-        lia.
-        lia.
-        lia.
-        lia.
-        lia.
-        lia. }
-    Qed.
 
-    Lemma split_p' : forall (p lo hi : list Z),
-        p = lo ++ hi ->
-        canonical_repr (2 * n) p ->
-        length lo = n ->
-        split (weight n) (combine (map weight (seq 0 n)) lo) = (combine (map weight (seq 0 n)) lo, []) /\
-          split (weight n) (combine (map weight (seq n n)) hi) = ([], combine (map weight (seq 0 n)) hi).
-    Proof.
-      intros.
-      intuition.
-      { apply split_lt.
-        intros.
-        rewrite in_map_iff in H2.
-        destruct H2.
-        intuition; rewrite <-H3.
+        (* not bounded *)
+        push.
+        ring_simplify.
+        rewrite <-Z_div_mod_eq.
         auto.
-        rewrite in_seq in H4.
-        apply weight_mono.
+        rewrite Z.gt_lt_iff.
+        auto.
+        push.
         lia.
-        rewrite map_length.
-        rewrite seq_length.
-        auto. }
-      { rewrite map_weight_seq with (m:=n).
-        apply split_gt.
-        intros.
-        rewrite in_map_iff in H2.
-        destruct H2.
-        intuition; rewrite <-H3.
-        apply Weight.weight_multiples_full.
-        auto.
-        auto.
-        rewrite in_seq in H4.
-        lia.
-        rewrite map_length, seq_length.
-        solve_length p. }
-    Qed.
+        push.
+      Qed.
+      Hint Rewrite eval_mul_no_reduce : push_eval.
 
-    Lemma reduce_first_canonical : forall (p lo hi : list Z),
-        p = lo ++ hi ->
-        canonical_repr (2 * n) p ->
-        length lo = n ->
-        canonical_repr (S n) (reduce1 base s c (2*n) (S n) p).
-    Proof.
-      intros.
-      unfold reduce1, canonical_repr.
-      split.
-      { rewrite Rows.flatten_correct.
-        cbn [fst].
-        auto with push_length.
-        auto.
+      Theorem length_mul_no_reduce : forall p q,
+          length (mul_no_reduce base n p q) = (2 * n)%nat.
+      Proof.
+        intros; unfold mul_no_reduce; break_match; push.
+      Qed.
+
+    End mul_no_reduce.
+
+    Section reduce1.
+
+      Lemma reduce1_length : forall p m1 m2,
+          length (reduce1 base s c m1 m2 p) = m2.
+      Proof.
+        intros; unfold reduce1; push.
+      Qed.
+      Hint Rewrite reduce1_length : push_length.
+
+    End reduce1.
+
+    Section reduce_first.
+
+      Lemma split_p : forall p lo hi,
+          p = lo ++ [hi] ->
+          canonical_repr (S n) p ->
+          (split (weight n) [(weight n, hi)] = ([], [(1, hi)])) /\
+            (split (weight n) (combine (map weight (seq 0 n)) lo) =
+               ((combine (map weight (seq 0 n)) lo), [])).
+      Proof.
         intros.
-        eapply Rows.length_from_associational; eauto. }
-      { pose proof (split_p' _ _ _ H H0 H1) as Hsplit.
+        intuition.
+        { intros.
+          unfold split.
+          simpl.
+          assert (weight n mod weight n = 0) by (apply Z_mod_same_full).
+          rewrite H1.
+          simpl.
+          assert (weight n / weight n = 1) by
+            auto using Z_div_same, Z.lt_gt, weight_positive.
+          rewrite H2.
+          reflexivity. }
+        { apply split_lt.
+          intros.
+          rewrite in_map_iff in H1.
+          destruct H1.
+          intuition.
+          rewrite <-H2.
+          auto.
+          rewrite <-H2.
+          rewrite in_seq in H3.
+          intuition.
+          simpl in H4.
+          apply weight_mono.
+          lia.
+          rewrite map_length.
+          rewrite seq_length.
+          solve_length p. }
+      Qed.
+
+      Lemma reduce_in_range : forall m x,
+          x < weight 1 - weight 0 ->
+          x + weight m < weight (S m).
+      Proof.
+        intros.
+        rewrite OrdersEx.Z_as_DT.lt_add_lt_sub_r.
+        induction m.
+        auto.
+        etransitivity.
+        apply IHm.
+        unfold weight.
+        rewrite uweight_S.
+        rewrite uweight_S.
+        rewrite <-uweight_S at 1.
+        rewrite <-OrdersEx.Z_as_OT.mul_sub_distr_l.
+        rewrite Z.mul_comm.
+        rewrite <-OrdersEx.Z_as_OT.lt_mul_diag_r.
+        simpl; lia.
+        rewrite OrdersEx.Z_as_OT.lt_0_sub.
+        fold weight.
+        apply weight_mono'.
+        lia.
+        lia.
+        lia.
+      Qed.
+
+      Lemma map_weight_seq : forall m p,
+          map weight (seq 0 p) = map (fun t => t / (weight m)) (map weight (seq m p)).
+      Proof.
+        induction m; intros.
+        { generalize dependent (map weight (seq 0 p)).
+          intros.
+          erewrite map_ext.
+          symmetry.
+          eapply map_id.
+          intros.
+          rewrite weight_0.
+          rewrite Z.div_1_r.
+          lia.
+          auto. }
+        { rewrite IHm.
+          push.
+          apply map_ext_Forall.
+          rewrite Forall_forall.
+          intros.
+          rewrite in_seq in H.
+          weight_comp; try lia.
+          rewrite <-!OrdersEx.Z_as_OT.pow_add_r; try lia.
+          rewrite <-!OrdersEx.Z_as_OT.pow_sub_r; try lia.
+          f_equal.
+          lia. }
+      Qed.
+
+      Lemma split_p' : forall (p lo hi : list Z),
+          p = lo ++ hi ->
+          canonical_repr (2 * n) p ->
+          length lo = n ->
+          split (weight n) (combine (map weight (seq 0 n)) lo) = (combine (map weight (seq 0 n)) lo, []) /\
+            split (weight n) (combine (map weight (seq n n)) hi) = ([], combine (map weight (seq 0 n)) hi).
+      Proof.
+        intros.
+        intuition.
+        { apply split_lt.
+          intros.
+          rewrite in_map_iff in H2.
+          destruct H2.
+          intuition; rewrite <-H3.
+          auto.
+          rewrite in_seq in H4.
+          apply weight_mono.
+          lia.
+          rewrite map_length.
+          rewrite seq_length.
+          auto. }
+        { rewrite map_weight_seq with (m:=n).
+          apply split_gt.
+          intros.
+          rewrite in_map_iff in H2.
+          destruct H2.
+          intuition; rewrite <-H3.
+          apply Weight.weight_multiples_full.
+          auto.
+          auto.
+          rewrite in_seq in H4.
+          lia.
+          rewrite map_length, seq_length.
+          solve_length p. }
+      Qed.
+
+      Lemma split_p_first_lo : forall p,
+          length p = (2 * n)%nat ->
+          split (weight n) (combine (map weight (seq 0 n)) (firstn n p)) = (combine (map weight (seq 0 n)) (firstn n p), []).
+      Proof.
+        intros p Hlen.
+        rewrite split_lt;
+          repeat multimatch goal with
+                 | H : _ |- _ => autorewrite with push_misc in H
+                 | H : _ |- _ => rewrite in_seq in H
+                 | _ => rewrite min_l
+                 | _ => rewrite map_weight_seq with (m:=n)
+                 | _ => apply Weight.weight_multiples_full
+                 | H : context[exists _, _] |- _ => destruct H
+                 | H : _ = ?x |- context[?x] => rewrite <-H
+                 | _ => unfold weight; rewrite <-uweight_sum_indices; fold weight
+                 | _ => push
+                 | _ => apply Z.div_lt_upper_bound
+                 | _ => apply Z.div_str_pos
+                 | _ => apply weight_mono
+                 | _ => apply weight_mono_le
+                 | _ => intuition
+                 | _ => auto || lia
+                 end.
+      Qed.
+      Hint Rewrite split_p_first_lo using auto : push_eval.
+
+      Lemma split_p_first_hi : forall p,
+          length p = (2 * n)%nat ->
+          split (weight n) (combine (map weight (seq n n)) (skipn n p)) = ([], combine (map weight (seq 0 n)) (skipn n p)).
+      Proof.
+        intros p Hlen.
+        rewrite split_gt;
+          repeat multimatch goal with
+                 | H : _ |- _ => autorewrite with push_misc in H
+                 | H : _ |- _ => rewrite in_seq in H
+                 | _ => rewrite min_l
+                 | _ => rewrite map_weight_seq with (m:=n)
+                 | _ => apply Weight.weight_multiples_full
+                 | H : context[exists _, _] |- _ => destruct H
+                 | H : _ = ?x |- context[?x] => rewrite <-H
+                 | _ => unfold weight; rewrite <-uweight_sum_indices; fold weight
+                 | _ => push
+                 | _ => apply Z.div_lt_upper_bound
+                 | _ => apply Z.div_str_pos
+                 | _ => apply weight_mono
+                 | _ => apply weight_mono_le
+                 | _ => intuition
+                 | _ => auto || lia
+                 end.
+      Qed.
+      Hint Rewrite split_p_first_hi using auto : push_eval.
+
+      Lemma value_reduce_first' : forall (p : list Z),
+          length p = (2 * n)%nat ->
+          let q := reduce1 base s c (2 * n) (S n) p in
+          let s' := fst (Saturated.Rows.adjust_s weight (S (S (S n))) s) in
+          let coef := Associational.sat_mul_const base [(1, s'/s)] c in
+          eval weight (S n) q = Associational.eval coef * eval weight n (skipn n p) + eval weight n (firstn n p).
+      Proof.
+        intros p Hlen ? ? ?.
+        cbv [q s' coef reduce1 to_associational].
+        pose proof (firstn_skipn n p) as Hp.
+        symmetry in Hp.
+        rewrite Hp.
+        push.
+        rewrite Hlen.
+        rewrite min_l; try lia.
+        erewrite !adjust_s_finished; try eapply solinas_property; try lia.
+        push.
+        rewrite skipn_all with (xs := firstn n p).
+        rewrite firstn_all with (xs := firstn n p).
+        push.
+        solve_ineq.
+        split;
+          solve_ineq.
+        all: admit.
+      Admitted.
+
+      Lemma value_reduce_first : forall (p lo hi : list Z),
+          p = lo ++ hi ->
+          canonical_repr (2 * n) p ->
+          length lo = n ->
+          let q := reduce1 base s c (2 * n) (S n) p in
+          let s' := fst (Saturated.Rows.adjust_s weight (S (S (S n))) s) in
+          let coef := Associational.sat_mul_const base [(1, s'/s)] c in
+          eval weight (S n) q = Associational.eval coef * eval weight n hi + eval weight n lo.
+      Proof.
+        intros.
+        pose proof (split_p' _ _ _ H H0 H1) as Hsplit.
         destruct Hsplit as [ Hlo Hhi ].
-        rewrite Rows.flatten_correct.
-        cbn [fst].
-        rewrite Partition.eval_partition.
-        f_equal.
-        apply Z.mod_small_sym.
-        rewrite Rows.eval_from_associational.
+        canonical_app p.
+        replace (length hi) with n in * by (solve_length p).
+        replace (length lo) with n in *.
+        unfold q, reduce1.
         rewrite H.
-        rewrite value_sat_reduce.
-        erewrite adjust_s_finished; try apply solinas_property.
+        rewrite Rows.flatten_mod, Rows.eval_from_associational, value_sat_reduce.
         unfold to_associational.
+        cbn [fst snd].
+        erewrite adjust_s_finished; try apply solinas_property.
         replace (2 * n)%nat with (n + n)%nat by lia.
         rewrite seq_add.
         rewrite Nat.add_0_l.
@@ -1385,15 +1277,16 @@ Finished transaction in 7.129 secs (6.859u,0.198s) (successful)
         cbn [fst snd].
         rewrite Hlo, Hhi.
         autorewrite with push_eval zsimplify_const.
+        cbn [snd].
+        unfold coef, s'.
+        autorewrite with push_eval zsimplify_const.
+        erewrite adjust_s_finished; try apply solinas_property.
         cbn [fst snd].
 
-        canonical_app p.
-        replace (length lo) with n in Hcanon_l by (solve_length p).
-        replace (length hi) with n in Hcanon_r.
+        rewrite Z.mod_small.
+        reflexivity.
         split.
-        solve_ineq.
-        apply canonical_pos; auto.
-        apply canonical_pos; auto.
+        solve_ineq; apply canonical_pos; auto.
         etransitivity.
         solve_ineq.
         apply Z.mul_lt_mono_nonneg.
@@ -1405,222 +1298,235 @@ Finished transaction in 7.129 secs (6.859u,0.198s) (successful)
         weight_comp.
         rewrite Z.mul_comm.
         rewrite Zred_factor3.
-        apply Zmult_lt_compat_l.
+        rewrite Z.mul_comm.
+        apply Zmult_lt_compat_r.
         lia.
-        simpl; lia.
+        simpl.
         lia.
         lia.
-        solve_length p.
-        rewrite map_length, seq_length; auto.
+        lia.
+        lia.
+        lia.
+        rewrite map_length, seq_length.
+        solve_length lo.
         lia.
         lia.
         lia.
         auto.
         lia.
         auto.
+        intros.
+        eapply Rows.length_from_associational; eauto.
+      Qed.
+
+      Lemma reduce_first_canonical : forall (p lo hi : list Z),
+          p = lo ++ hi ->
+          canonical_repr (2 * n) p ->
+          length lo = n ->
+          canonical_repr (S n) (reduce1 base s c (2*n) (S n) p).
+      Proof.
+        intros.
+        unfold reduce1, canonical_repr.
+        split.
+        { rewrite Rows.flatten_correct.
+          cbn [fst].
+          auto with push_length.
+          auto.
+          intros.
+          eapply Rows.length_from_associational; eauto. }
+        { pose proof (split_p' _ _ _ H H0 H1) as Hsplit.
+          destruct Hsplit as [ Hlo Hhi ].
+          rewrite Rows.flatten_correct.
+          cbn [fst].
+          rewrite Partition.eval_partition.
+          f_equal.
+          apply Z.mod_small_sym.
+          rewrite Rows.eval_from_associational.
+          rewrite H.
+          rewrite value_sat_reduce.
+          erewrite adjust_s_finished; try apply solinas_property.
+          unfold to_associational.
+          replace (2 * n)%nat with (n + n)%nat by lia.
+          rewrite seq_add.
+          rewrite Nat.add_0_l.
+          rewrite map_app.
+          rewrite combine_app_samelength.
+          rewrite fst_split_app, snd_split_app.
+          cbn [fst snd].
+          rewrite Hlo, Hhi.
+          autorewrite with push_eval zsimplify_const.
+          cbn [fst snd].
+
+          canonical_app p.
+          replace (length lo) with n in Hcanon_l by (solve_length p).
+          replace (length hi) with n in Hcanon_r.
+          split.
+          solve_ineq.
+          apply canonical_pos; auto.
+          apply canonical_pos; auto.
+          etransitivity.
+          solve_ineq.
+          apply Z.mul_lt_mono_nonneg.
+          solve_ineq.
+          eauto.
+          apply canonical_pos; auto.
+          apply canonical_eval_bounded; auto.
+          apply canonical_eval_bounded; auto.
+          weight_comp.
+          rewrite Z.mul_comm.
+          rewrite Zred_factor3.
+          rewrite Z.mul_comm.
+          apply Zmult_lt_compat_r.
+          lia.
+          simpl; lia.
+          lia.
+          lia.
+          solve_length p.
+          rewrite map_length, seq_length; auto.
+          lia.
+          lia.
+          lia.
+          auto.
+          lia.
+          auto.
+          auto.
+          eapply Rows.length_from_associational; eauto. }
+      Qed.
+
+      Lemma reduce_first : forall (p lo hi : list Z),
+          p = lo ++ hi ->
+          canonical_repr (2 * n) p ->
+          length lo = n ->
+          forall q_lo q_hi,
+            let q := reduce1 base s c (2*n) (S n) p in
+            q = q_lo ++ [q_hi] ->
+            q_hi < up_bound.
+      Proof.
+        intros.
+        pose proof (value_reduce_first _ _ _ H H0 H1).
+        pose proof (reduce_first_canonical _ _ _ H H0 H1) as Hcanon.
+        fold q in Hcanon.
+
+        pose proof fun pf => nth_default_partition weight 0 (S n) (eval weight (S n) q) (n) pf as Hnth.
+        assert (Hcanon' := Hcanon).
+        unfold canonical_repr in Hcanon'.
+        destruct Hcanon' as [ _ Hpart ].
+        rewrite <-Hpart in Hnth.
+        rewrite H2 in Hnth at 1.
+        rewrite nth_default_app in Hnth.
+        destruct lt_dec in Hnth.
+        solve_length q.
+        replace (length q_lo) with n in Hnth by (solve_length q).
+        rewrite Nat.sub_diag in Hnth.
+        unfold nth_default in Hnth.
+        simpl in Hnth.
+        rewrite Hnth.
+        unfold q.
+        apply Z.div_lt_upper_bound.
         auto.
-        eapply Rows.length_from_associational; eauto. }
-    Qed.
 
-    Lemma value_reduce_first : forall (p lo hi : list Z),
-        p = lo ++ hi ->
-        canonical_repr (2 * n) p ->
-        length lo = n ->
-        let q := reduce1 base s c (2 * n) (S n) p in
-        let s' := fst (Saturated.Rows.adjust_s weight (S (S (S n))) s) in
-        let coef := Associational.sat_mul_const base [(1, s'/s)] c in
-        eval weight (S n) q = Associational.eval coef * eval weight n hi + eval weight n lo.
-    Proof.
-      intros.
-      pose proof (split_p' _ _ _ H H0 H1) as Hsplit.
-      destruct Hsplit as [ Hlo Hhi ].
-      canonical_app p.
-      replace (length hi) with n in * by (solve_length p).
-      replace (length lo) with n in *.
-      unfold q, reduce1.
-      rewrite H.
-      rewrite Rows.flatten_mod, Rows.eval_from_associational, value_sat_reduce.
-      unfold to_associational.
-      cbn [fst snd].
-      erewrite adjust_s_finished; try apply solinas_property.
-      replace (2 * n)%nat with (n + n)%nat by lia.
-      rewrite seq_add.
-      rewrite Nat.add_0_l.
-      rewrite map_app.
-      rewrite combine_app_samelength.
-      rewrite fst_split_app, snd_split_app.
-      cbn [fst snd].
-      rewrite Hlo, Hhi.
-      autorewrite with push_eval zsimplify_const.
-      cbn [snd].
-      unfold coef, s'.
-      autorewrite with push_eval zsimplify_const.
-      erewrite adjust_s_finished; try apply solinas_property.
-      cbn [fst snd].
+        canonical_app p.
+        replace (length lo) with n in Hcanon_l.
+        replace (length hi) with n in Hcanon_r by (solve_length p).
+        rewrite H3.
+        autorewrite with push_eval zsimplify_const.
+        erewrite adjust_s_finished; try apply solinas_property.
+        cbn [fst snd].
+        rewrite <-Le.Z.le_sub_1_iff.
+        rewrite Z.mod_small.
+        etransitivity.
+        solve_ineq.
+        rewrite <-Le.Z.le_sub_1_iff in coef_small.
+        apply Z.mul_le_mono_nonneg.
+        solve_ineq.
+        eauto.
+        apply canonical_pos; auto.
+        rewrite Le.Z.le_sub_1_iff.
+        eapply canonical_eval_bounded; auto.
+        rewrite Le.Z.le_sub_1_iff.
+        apply canonical_eval_bounded; auto.
+        ring_simplify.
+        rewrite OrdersEx.Z_as_OT.le_sub_le_add_r.
+        unfold up_bound.
+        weight_comp.
+        simpl.
+        nia.
 
-      rewrite Z.mod_small.
-      reflexivity.
-      split.
-      solve_ineq; apply canonical_pos; auto.
-      etransitivity.
-      solve_ineq.
-      apply Z.mul_lt_mono_nonneg.
-      solve_ineq.
-      eauto.
-      apply canonical_pos; auto.
-      apply canonical_eval_bounded; auto.
-      apply canonical_eval_bounded; auto.
-      weight_comp.
-      rewrite Z.mul_comm.
-      rewrite Zred_factor3.
-      apply Zmult_lt_compat_l.
-      lia.
-      simpl.
-      lia.
-      lia.
-      lia.
-      lia.
-      lia.
-      rewrite map_length, seq_length.
-      solve_length lo.
-      lia.
-      lia.
-      lia.
-      auto.
-      lia.
-      auto.
-      intros.
-      eapply Rows.length_from_associational; eauto.
-    Qed.
+        split.
+        solve_ineq.
+        apply canonical_pos; auto.
+        apply canonical_pos; auto.
+        etransitivity.
+        solve_ineq.
+        apply Z.mul_lt_mono_nonneg.
+        solve_ineq.
+        eauto.
+        apply canonical_pos; auto.
+        eapply canonical_eval_bounded; auto.
+        eapply canonical_eval_bounded; auto.
+        weight_comp.
+        unfold up_bound, machine_wordsize.
+        rewrite Z.mul_comm.
+        rewrite Zred_factor3.
+        rewrite Z.mul_comm.
+        apply Zmult_lt_compat_r.
+        lia.
+        cbn.
+        lia.
+        lia.
+        lia.
+        lia.
+        lia.
+        lia.
+      Qed.
 
-    Lemma reduce_first : forall (p lo hi : list Z),
-        p = lo ++ hi ->
-        canonical_repr (2 * n) p ->
-        length lo = n ->
-        forall q_lo q_hi,
-          let q := reduce1 base s c (2*n) (S n) p in
-          q = q_lo ++ [q_hi] ->
-          q_hi < up_bound.
-    Proof.
-      intros.
-      pose proof (value_reduce_first _ _ _ H H0 H1).
-      pose proof (reduce_first_canonical _ _ _ H H0 H1) as Hcanon.
-      fold q in Hcanon.
+      Lemma reduce_first_correct : forall (p lo hi : list Z),
+          p = lo ++ hi ->
+          canonical_repr (2 * n) p ->
+          length lo = n ->
+          let q := reduce1 base s c (2 * n) (S n) p in
+          (Positional.eval weight (2 * n) p) mod (s - Associational.eval c)
+          = (Positional.eval weight (S n) q) mod (s - Associational.eval c).
+      Proof.
+        intros.
+        pose proof (value_reduce_first _ _ _ H H0 H1) as Hval.
+        canonical_app p.
+        replace (length hi) with n in Hcanon_r by (solve_length p).
+        replace (length lo) with n in Hcanon_l.
+        unfold q in *.
+        rewrite Hval.
+        rewrite H.
+        unfold weight.
+        replace (2 * n)%nat with (n + (length hi))%nat by (solve_length p).
+        rewrite uweight_eval_app'.
+        replace (length hi) with n by (solve_length hi).
+        fold weight.
+        autorewrite with push_eval zsimplify_const.
+        erewrite adjust_s_finished'; try apply solinas_property.
+        cbn [fst snd].
+        rewrite (Z.add_comm _ (eval weight n lo)).
+        rewrite Z.mul_comm with (m:=Associational.eval c).
+        rewrite <-Z.mul_assoc.
+        rewrite <-reduction_rule.
+        apply Z.elim_mod.
+        rewrite Z.add_cancel_l.
+        rewrite Z.mul_assoc.
+        rewrite <-Z_div_exact_2.
+        lia.
+        lia.
+        pose proof (adjust_s_invariant (S (S (S n))) s) as Hinv.
+        erewrite adjust_s_finished' in Hinv; try apply solinas_property.
+        cbn [fst] in Hinv.
+        apply Hinv.
+        lia.
+        lia.
+        lia.
+        lia.
+        lia.
+        solve_length lo.
+      Qed.
 
-      pose proof fun pf => nth_default_partition weight 0 (S n) (eval weight (S n) q) (n) pf as Hnth.
-      assert (Hcanon' := Hcanon).
-      unfold canonical_repr in Hcanon'.
-      destruct Hcanon' as [ _ Hpart ].
-      rewrite <-Hpart in Hnth.
-      rewrite H2 in Hnth at 1.
-      rewrite nth_default_app in Hnth.
-      destruct lt_dec in Hnth.
-      solve_length q.
-      replace (length q_lo) with n in Hnth by (solve_length q).
-      rewrite Nat.sub_diag in Hnth.
-      unfold nth_default in Hnth.
-      simpl in Hnth.
-      rewrite Hnth.
-      unfold q.
-      apply Z.div_lt_upper_bound.
-      auto.
-
-      canonical_app p.
-      replace (length lo) with n in Hcanon_l.
-      replace (length hi) with n in Hcanon_r by (solve_length p).
-      rewrite H3.
-      autorewrite with push_eval zsimplify_const.
-      erewrite adjust_s_finished; try apply solinas_property.
-      cbn [fst snd].
-      rewrite <-Le.Z.le_sub_1_iff.
-      rewrite Z.mod_small.
-      etransitivity.
-      solve_ineq.
-      rewrite <-Le.Z.le_sub_1_iff in coef_small.
-      apply Z.mul_le_mono_nonneg.
-      solve_ineq.
-      eauto.
-      apply canonical_pos; auto.
-      rewrite Le.Z.le_sub_1_iff.
-      eapply canonical_eval_bounded; auto.
-      rewrite Le.Z.le_sub_1_iff.
-      apply canonical_eval_bounded; auto.
-      ring_simplify.
-      rewrite OrdersEx.Z_as_OT.le_sub_le_add_r.
-      unfold up_bound.
-      weight_comp.
-      simpl.
-      nia.
-
-      split.
-      solve_ineq.
-      apply canonical_pos; auto.
-      apply canonical_pos; auto.
-      etransitivity.
-      solve_ineq.
-      apply Z.mul_lt_mono_nonneg.
-      solve_ineq.
-      eauto.
-      apply canonical_pos; auto.
-      eapply canonical_eval_bounded; auto.
-      eapply canonical_eval_bounded; auto.
-      weight_comp.
-      unfold up_bound, machine_wordsize.
-      simpl.
-      break_match; try lia.
-      destruct Heqz; break_match; lia.
-      lia.
-      lia.
-      lia.
-      lia.
-      lia.
-    Qed.
-
-    Lemma reduce_first_correct : forall (p lo hi : list Z),
-        p = lo ++ hi ->
-        canonical_repr (2 * n) p ->
-        length lo = n ->
-        let q := reduce1 base s c (2 * n) (S n) p in
-        (Positional.eval weight (2 * n) p) mod (s - Associational.eval c)
-        = (Positional.eval weight (S n) q) mod (s - Associational.eval c).
-    Proof.
-      intros.
-      pose proof (value_reduce_first _ _ _ H H0 H1) as Hval.
-      canonical_app p.
-      replace (length hi) with n in Hcanon_r by (solve_length p).
-      replace (length lo) with n in Hcanon_l.
-      unfold q in *.
-      rewrite Hval.
-      rewrite H.
-      unfold weight.
-      replace (2 * n)%nat with (n + (length hi))%nat by (solve_length p).
-      rewrite uweight_eval_app'.
-      replace (length hi) with n by (solve_length hi).
-      fold weight.
-      autorewrite with push_eval zsimplify_const.
-      erewrite adjust_s_finished'; try apply solinas_property.
-      cbn [fst snd].
-      rewrite (Z.add_comm _ (eval weight n lo)).
-      rewrite Z.mul_comm with (m:=Associational.eval c).
-      rewrite <-Z.mul_assoc.
-      rewrite <-reduction_rule.
-      apply Z.elim_mod.
-      rewrite Z.add_cancel_l.
-      rewrite Z.mul_assoc.
-      rewrite <-Z_div_exact_2.
-      lia.
-      lia.
-      pose proof (adjust_s_invariant (S (S (S n))) s) as Hinv.
-      erewrite adjust_s_finished' in Hinv; try apply solinas_property.
-      cbn [fst] in Hinv.
-      apply Hinv.
-      lia.
-      lia.
-      lia.
-      lia.
-      lia.
-      solve_length lo.
-    Qed.
+    End reduce_first.
 
     Lemma reduce_second_canonical : forall (p : list Z) lo hi,
         p = lo ++ [hi] ->
@@ -2632,13 +2538,14 @@ Finished transaction in 7.129 secs (6.859u,0.198s) (successful)
     Admitted.
 
     Theorem mulmod_correct : forall p q,
-        canonical_repr n p ->
-        canonical_repr n q ->
         Positional.eval weight n (mulmod base s c n p q) mod (s - Associational.eval c) =
           (Positional.eval weight n p * Positional.eval weight n q) mod (s - Associational.eval c).
     Proof.
       intros.
-
+      unfold mulmod.
+      rewrite <-reduce_full_correct.
+      rewrite <-eval_mul_no_reduce.
+      auto.
       admit.
     Admitted.
 
